@prefix rdf:    <http://www.w3.org/1999/02/22-rdf-syntax-ns#> .
@prefix rdfs:   <http://www.w3.org/2000/01/rdf-schema#> .
@prefix owl:    <http://www.w3.org/2002/07/owl#> .
@prefix cc:     <http://creativecommons.org/ns#> .
@prefix xsd:    <http://www.w3.org/2001/XMLSchema#> .
@prefix dct:    <http://purl.org/dc/terms/> .
@prefix vann:   <http://purl.org/vocab/vann/> .
@prefix foaf:   <http://xmlns.com/foaf/0.1/> .
@prefix qudt:   <http://qudt.org/schema/qudt/> .
@prefix unit:   <http://qudt.org/vocab/unit/> .
@prefix opp:    <https://w3id.org/openplannerteam/profile#> .

# About

<https://w3id.org/openplannerteam/profile>
        a                 foaf:Document ;
        foaf:primaryTopic opp: .

opp:    a                              owl:Ontology ;
        dct:description                """This ontology describes the OpenPlanner profile data model.
                                          It currently supports: 
                                            i) setting a default maximum speed,
                                            ii) whether or not to use public transportation, 
                                            iii) describing which roads are accessible,
                                            iv) describing which nodes are obstacles,
                                            v) describing which roads are oneway streets,
                                            vi) describing which roads should be given priority, and
                                            vii) describing the maximum speed for a road."""@en ;
        cc:license                     <https://creativecommons.org/licenses/by/4.0/> ;
        rdfs:label                     "OpenPlanner Profile Vocabulary"@en ;
        vann:preferredNamespacePrefix  "opp" ;
        vann:preferredNamespaceUri     "https://w3id.org/openplannerteam/profile#" ;
        dct:creator                    <https://biblio.ugent.be/person/802002413821> ;
        dct:creator                    <https://pietercolpaert.be/#me> ;
        dct:issued                     "2019-06-14"^^xsd:date ;
        dct:modified                   "2019-06-18"^^xsd:date .

<https://biblio.ugent.be/person/802002413821> 
        a                 foaf:Person ;
        foaf:name         "Harm Delva" ;
        foaf:mbox         "harm.delva@ugent.be" .


# Element Classes

opp:Profile  
        a                     rdfs:Class , owl:Class ;
        rdfs:label            "Profile"@en ;
        rdfs:comment          """Combines sets of rules and some default values.""" ;
        owl:disjointWith      opp:Condition , opp:Rule;
        rdfs:isDefinedBy      opp: .

opp:Rule  
        a                     rdfs:Class , owl:Class ;
        rdfs:label            "Rule"@en ;
        rdfs:comment          """The core element of a profile, it defines a condition that must be met to make a conclusion.
                                 The condition may be empty, which means that the rule always applies.""" ;
        owl:disjointWith      opp:Condition , opp:Profile ;
        rdfs:isDefinedBy      opp: .

opp:Condition  
        a                     rdfs:Class , owl:Class ;
        rdfs:label            "Condition"@en ;
        rdfs:comment          "Defines a condition that must be must for a rule to apply." ;
        owl:disjointWith      opp:Rule , opp:Profile ;
        rdfs:isDefinedBy      opp: .

# Object Properties

opp:match
        a                     owl:ObjectProperty , rdf:Property ;
        owl:minCardinality    0;
        rdfs:comment          "Describes a condition to match."@en ;
        rdfs:label            "match"@en ;
        rdfs:isDefinedBy      opp: ;
        rdfs:domain           opp:Rule ;
        rdfs:range            opp:Condition .

opp:hasPredicate
        a                     owl:ObjectProperty , rdf:Property ;
        owl:minCardinality    0;
        rdfs:comment          "Match things with this specific predicate (key)."@en ;
        rdfs:label            "hasPredicate"@en ;
        rdfs:isDefinedBy      opp: ;
        rdfs:domain           opp:Condition .

opp:hasObject
        a                     owl:ObjectProperty , rdf:Property ;
        owl:minCardinality    0;
        rdfs:comment          "Match things with this specific object (value)."@en ;
        rdfs:label            "hasObject"@en ;
        rdfs:isDefinedBy      opp: ;
        rdfs:domain           opp:Condition .

opp:fromProperty
        a                     owl:ObjectProperty , rdf:Property ;
        owl:cardinality       1;
        rdfs:comment          "Copy the value that corresponds with this key."@en ;
        rdfs:label            "fromProperty"@en ;
        rdfs:isDefinedBy      opp: .

opp:hasAccessRules
        a                     owl:ObjectProperty , rdf:Property ;
        owl:maxCardinality    1;
        rdfs:comment          "An ordered list of rules that determines whether or not a way is accessible. Only the first rule that matches will be used."@en ;
        rdfs:label            "hasAccessRules"@en ;
        rdfs:isDefinedBy      opp: ;
        rdfs:domain           opp:Profile ;
        rdfs:range            opp:Rule .

opp:hasOnewayRules
        a                     owl:ObjectProperty , rdf:Property ;
        owl:maxCardinality    1;
        rdfs:comment          "An ordered list of rules that determines whether or not something is a oneway street. Only the first rule that matches will be used."@en ;
        rdfs:label            "hasOnewayRules"@en ;
        rdfs:isDefinedBy      opp: ;
        rdfs:domain           opp:Profile ;
        rdfs:range            opp:Rule .

opp:hasSpeedRules
        a                     owl:ObjectProperty , rdf:Property ;
        owl:maxCardinality    1;
        rdfs:comment          "An ordered list of rules that determines the maximum speed on a street. Only the first rule that matches will be used."@en ;
        rdfs:label            "hasSpeedRules"@en ;
        rdfs:isDefinedBy      opp: ;
        rdfs:domain           opp:Profile ;
        rdfs:range            opp:Rule .

opp:hasPriorityRules
        a                     owl:ObjectProperty , rdf:Property ;
        owl:maxCardinality    1;
        rdfs:comment          "An ordered list of rules that determines an additional multiplier that will be used to demote/promote certain roads. Only the first rule that matches will be used."@en ;
        rdfs:label            "hasPriorityRules"@en ;
        rdfs:isDefinedBy      opp: ;
        rdfs:domain           opp:Profile ;
        rdfs:range            opp:Rule .

opp:hasObstacleRules
        a                     owl:ObjectProperty , rdf:Property ;
        owl:maxCardinality    1;
        rdfs:comment          "An ordered list of rules that determines whether or not a node can be traversed. Only the first rule that matches will be used."@en ;
        rdfs:label            "hasObstacleRules"@en ;
        rdfs:isDefinedBy      opp: ;
        rdfs:domain           opp:Profile ;
        rdfs:range            opp:Rule .

# Data properties

opp:concludes
        a                     owl:DatatypeProperty , rdf:Property ;
        rdfs:comment          "Describes a conclusion that can be made after matching a rule."@en ;
        rdfs:label            "conclude"@en ;
        rdfs:isDefinedBy      opp: ;
        rdfs:domain           opp:Rule .

opp:hasMaxSpeed
        a                     owl:DatatypeProperty , rdf:Property ;
        rdfs:subPropertyOf    opp:concludes ;
        rdfs:comment          "The maximum legal or physical speed, in km/h."@en ;
        rdfs:label            "hasMaxSpeed"@en ;
        rdfs:isDefinedBy      opp: ;
        qudt:hasUnit          unit:KM-PER-HR ;
        rdfs:domain           opp:Rule ;
        rdfs:range            xsd:double .

opp:usePublicTransport
        a                     owl:DatatypeProperty , rdf:Property ;
        rdfs:comment          "Should public transportation be used."@en ;
        rdfs:label            "usePublicTransport"@en ;
        rdfs:isDefinedBy      opp: ;
        rdfs:domain           opp:Profile ;
        rdfs:range            xsd:boolean .

opp:hasAccess
        a                     owl:DatatypeProperty , rdf:Property ;
        rdfs:subPropertyOf    opp:concludes ;
        rdfs:comment          "Is a street accessible?"@en ;
        rdfs:label            "hasAccess"@en ;
        rdfs:isDefinedBy      opp: ;
        rdfs:domain           opp:Rule ;
        rdfs:range            xsd:boolean .

opp:isOneway
        a                     owl:DatatypeProperty , rdf:Property ;
        rdfs:subPropertyOf    opp:concludes ;
        rdfs:comment          "Is it a oneway street?"@en ;
        rdfs:label            "isOneway"@en ;
        rdfs:isDefinedBy      opp: ;
        rdfs:domain           opp:Rule ;
        rdfs:range            xsd:boolean .

opp:isReversed
        a                     owl:DatatypeProperty , rdf:Property ;
        rdfs:subPropertyOf    opp:concludes ;
        rdfs:comment          "If it is a oneway street, should the direction of the nodes be reversed?"@en ;
        rdfs:label            "isReversed"@en ;
        rdfs:isDefinedBy      opp: ;
        rdfs:domain           opp:Rule ;
        rdfs:range            xsd:boolean .

opp:hasSpeed
        a                     owl:DatatypeProperty , rdf:Property ;
        rdfs:subPropertyOf    opp:concludes ;
        rdfs:label            "hasSpeed"@en ;
        rdfs:comment          "The default speed on a road, in km/h."@en ;
        rdfs:isDefinedBy      opp: ;
        rdfs:domain           opp:Rule ;
        rdfs:range            xsd:double .

opp:hasPriority
        a                     owl:DatatypeProperty , rdf:Property ;
        rdfs:subPropertyOf    opp:concludes ;
        rdfs:label            "hasPriority"@en ;
        rdfs:comment          "A multiplier that is used to promote/demote roads. A value larger than 1 will promote a road."@en ;
        rdfs:isDefinedBy      opp: ;
        rdfs:domain           opp:Rule ;
        rdfs:range            xsd:double .

opp:isObstacle
        a                     owl:DatatypeProperty , rdf:Property ;
        rdfs:subPropertyOf    opp:concludes ;
        rdfs:label            "isObstacle"@en ;
        rdfs:comment          "Is a node an obstacle?"@en ;
        rdfs:isDefinedBy      opp: ;
        rdfs:domain           opp:Rule ;
        rdfs:range            xsd:boolean .
